Learn.LowStar.List.Data.fst
@@ -1,0 +1,340 @@
+module Learn.LowStar.List.Data
+
+module L   = FStar.List.Pure
+module Ll  = Learn.List
+module B   = LowStar.Buffer
+module M   = LowStar.Modifies
+module G   = FStar.Ghost
+module T   = FStar.Tactics
+module HS  = FStar.HyperStack
+module ST  = FStar.HyperStack.ST
+
+open LowStar.BufferOps
+open FStar.HyperStack.ST
+
+
+#push-options "--__no_positivity"
+noeq
+type t (a: Type0) =
+  B.pointer_or_null (cell a)
+and cell (a: Type0) = {
+  next: t a;
+  data: a;
+}
+#pop-options
+
+noeq
+type list_seg (a : Type0) = {
+  segment : list (B.pointer (cell a) & a);
+  exit    : t a;
+}
+
+let list_nil (a : Type0) : Type = sg:list_seg a{sg.exit == B.null}
+
+
+unfold let sg_v (#a : Type0) (sg : list_seg a) : Tot (list a)
+  = L.map snd sg.segment
+
+unfold let sg_length (#a : Type0) (sg : list_seg a) : Tot nat
+  = L.length sg.segment
+
+let sg_cell (#a : Type0) (sg : list_seg a) (i : nat)
+  : Ghost (B.pointer (cell a)) (requires i < sg_length sg) (ensures fun _ -> True)
+  = (L.index sg.segment i)._1
+
+let entry (#a : Type0) (sg : list_seg a) : Tot (t a)
+  = if Nil? sg.segment then sg.exit else (L.hd sg.segment)._1
+
+unfold let tail_seg (#a : Type0) (sg : list_seg a)
+  : Pure (list_seg a) (requires Cons? sg.segment) (ensures fun _ -> True)
+  = {sg with segment = L.tail sg.segment}
+
+(** Pédicats *)
+
+let rec loc_seg (#a : Type) (sg : list_seg a) : GTot M.loc
+  (decreases sg.segment)
+  = match sg.segment with
+    | [] -> M.loc_none
+    | hd :: tl -> M.(loc_union (loc_buffer hd._1) (loc_seg (tail_seg sg)))
+
+(* Utiliser uniquement cette version ? *)
+let rec loc_addr_seg (#a : Type) (sg : list_seg a) : GTot M.loc
+  (decreases sg.segment)
+  = match sg.segment with
+    | [] -> M.loc_none
+    | hd :: tl -> M.(loc_union (loc_addr_of_buffer hd._1) (loc_addr_seg (tail_seg sg)))
+
+let rec wf_seg (#a : Type) (sg : list_seg a) : Tot prop
+  (decreases sg.segment)
+  = match sg.segment with
+    | [] -> True
+    | hd :: tl -> (M.loc_disjoint (B.loc_buffer hd._1) (loc_seg (tail_seg sg)))
+             /\ wf_seg (tail_seg sg)
+
+let rec wf_addr_seg (#a : Type) (sg : list_seg a) : Tot prop
+  (decreases sg.segment)
+  = match sg.segment with
+    | [] -> True
+    | hd :: tl -> (M.loc_disjoint (B.loc_addr_of_buffer hd._1) (loc_addr_seg (tail_seg sg)))
+             /\ wf_addr_seg (tail_seg sg)
+
+let freeable_seg (#a : Type) (sg : list_seg a) : Tot prop
+  = Ll.g_for_allP sg.segment (fun x -> B.freeable x._1)
+
+let rec live_seg (#a : Type) (h : HS.mem) (sg : list_seg a) : Tot prop
+  (decreases sg.segment)
+  = match sg.segment with
+    | [] -> True
+    | hd :: tl -> let sg' = tail_seg sg in 
+               B.live h hd._1 /\ B.deref h hd._1 == {next = entry sg'; data = hd._2} /\ live_seg h sg'
+
+
+(** Lemmes sur les prédicats *)
+
+let rec loc_seg_live_in (#a : Type) (h : HS.mem) (sg : list_seg a)
+  : Lemma (requires live_seg h sg) (ensures B.loc_in (loc_seg sg) h)
+          (decreases sg.segment)
+    [SMTPat (live_seg h sg)]
+  = match sg.segment with
+    | [] -> ()
+    | _ :: _ -> loc_seg_live_in h (tail_seg sg)
+
+let rec loc_addr_seg_live_in (#a : Type) (h : HS.mem) (sg : list_seg a)
+  : Lemma (requires live_seg h sg) (ensures B.loc_in (loc_addr_seg sg) h)
+          (decreases sg.segment)
+  = match sg.segment with
+    | [] -> ()
+    | _ :: _ -> loc_addr_seg_live_in h (tail_seg sg)
+
+let rec loc_addr_seg_includes (#a : Type) (sg : list_seg a)
+  : Lemma (ensures M.loc_includes (loc_addr_seg sg) (loc_seg sg))
+          (decreases sg.segment)
+  = match sg.segment with
+    | [] -> ()
+    | _ :: _ -> loc_addr_seg_includes (tail_seg sg)
+
+
+let rec loc_seg_includes_cell (#a : Type) (sg : list_seg a) (i : nat)
+  : Lemma (requires  i < sg_length sg)
+          (ensures   M.(loc_includes (loc_seg sg) (loc_buffer (sg_cell sg i))))
+          (decreases i)
+          [SMTPat (sg_cell sg i); SMTPat (loc_seg sg)]
+  = if i = 0 then () else loc_seg_includes_cell (tail_seg sg) (i - 1)
+
+let loc_union_comm12 (s0 s1 s2 : M.loc)
+  : Lemma M.(loc_union s0 (loc_union s1 s2) == loc_union s1 (loc_union s0 s2))
+  = M.(loc_union_assoc s0 s1 s2; loc_union_comm s0 s1; loc_union_assoc s1 s0 s2)
+
+let loc_seg_fold_f #a (c : B.pointer (cell a) & a) : M.loc -> GTot M.loc
+  = M.(loc_union (loc_buffer c._1))
+
+let loc_seg_fold_f_comm a :
+  Lemma (ensures Ll.fold_right_gtot_f_comm (loc_seg_fold_f #a))
+  = let f = loc_seg_fold_f #a in
+    introduce forall x0 x1 y . f x0 (f x1 y) == f x1 (f x0 y)
+      with loc_union_comm12 M.(loc_buffer x0._1) M.(loc_buffer x1._1) y
+
+let rec loc_seg_fold (#a : Type) (sg : list_seg a)
+  : Lemma (ensures loc_seg sg == L.fold_right_gtot sg.segment loc_seg_fold_f M.loc_none)
+          (decreases sg.segment)
+  = match sg.segment with
+    | [] -> ()
+    | _ :: _ -> loc_seg_fold (tail_seg sg)
+
+let rec frame (#a : Type) (h0 h1 : HS.mem) (sg : list_seg a) (r : B.loc)
+  : Lemma (requires live_seg h0 sg /\ M.(modifies r h0 h1 /\ loc_disjoint r (loc_seg sg)))
+          (ensures  live_seg h1 sg)
+          (decreases sg.segment)
+    [SMTPat (live_seg #a h0 sg); SMTPat (M.modifies r h0 h1)]
+    (* or [SMTPat (M.modifies r h0 h1); SMTPat (live_seg #a h1 sg)] ? *)
+  = match sg.segment with
+    | [] -> ()
+    | hd :: tl -> frame h0 h1 (tail_seg sg) r
+
+
+(** opérations *)
+
+(* [push_seg] *)
+
+let push_seg (#a : Type0) (p : B.pointer (cell a)) (x : a) (sg : list_seg a) : list_seg a
+  = { sg with segment = (p,x) :: sg.segment }
+
+(* [append_seg] *)
+
+let append_seg (#a : Type0) (sg0 sg1 : list_seg a) : Tot (list_seg a)
+  = { segment = L.(sg0.segment @ sg1.segment);
+      exit    = sg1.exit }
+
+let append_seg_assoc (#a : Type) (sg0 sg1 sg2 : list_seg a)
+  : Lemma (ensures append_seg sg0 (append_seg sg1 sg2) == append_seg (append_seg sg0 sg1) sg2)
+  = L.append_assoc sg0.segment sg1.segment sg2.segment
+
+let rec append_seg_loc (#a : Type) (sg0 sg1 : list_seg a)
+  : Lemma (ensures loc_seg (append_seg sg0 sg1) == M.loc_union (loc_seg sg0) (loc_seg sg1))
+          (decreases sg0.segment)
+          [SMTPat (loc_seg (append_seg sg0 sg1))]
+  = match sg0.segment with
+    | [] -> ()
+    | hd :: _ ->
+      append_seg_loc (tail_seg sg0) sg1;
+      M.loc_union_assoc (M.loc_buffer hd._1) (loc_seg (tail_seg sg0)) (loc_seg sg1)
+
+let rec append_seg_wf (#a : Type) (sg0 sg1 : list_seg a)
+  : Lemma (ensures wf_seg (append_seg sg0 sg1) <==>
+                   wf_seg sg0 /\ wf_seg sg1 /\ M.loc_disjoint (loc_seg sg0) (loc_seg sg1))
+          (decreases sg0.segment)
+          [SMTPat (wf_seg (append_seg sg0 sg1))]
+  = match sg0.segment with
+    | [] -> ()
+    | _ :: _ -> append_seg_wf (tail_seg sg0) sg1
+
+let rec append_seg_live (#a : Type) (h : HS.mem) (sg0 sg1 : list_seg a)
+  : Lemma (requires sg0.exit == entry sg1)
+          (ensures live_seg h (append_seg sg0 sg1) <==> live_seg h sg0 /\ live_seg h sg1)
+          (decreases sg0.segment)
+          [SMTPat (live_seg h (append_seg sg0 sg1))]
+  = match sg0.segment with
+    | [] -> ()
+    | _ :: _ -> append_seg_live h (tail_seg sg0) sg1
+
+(* [insert_seg] *)
+
+let insert_seg (#a : Type0) (i : nat) (x : B.pointer (cell a) & a) (sg : list_seg a)
+  : Pure (list_seg a) (requires i <= sg_length sg) (ensures fun _ -> True)
+  = { sg with segment = Ll.insert i x sg.segment }
+
+let rec insert_seg_loc (#a : Type) (i : nat) (x : B.pointer (cell a) & a) (sg : list_seg a)
+  : Lemma (requires i <= sg_length sg)
+          (ensures loc_seg (insert_seg i x sg) == M.(loc_union (loc_buffer x._1) (loc_seg sg)))
+          (decreases i)
+          [SMTPat (loc_seg (insert_seg i x sg))]
+  = if i = 0 then ()
+    else begin let hd = (L.hd sg.segment)._1 in
+         insert_seg_loc (i - 1) x (tail_seg sg);
+         M.(loc_union_comm12 (loc_buffer hd) (loc_buffer x._1) (loc_seg (tail_seg sg)))
+    end
+
+(* [splitAt_seg] *)
+
+let splitAt_seg (#a:Type) (n:nat) (sg:list_seg a) : Tot (list_seg a & list_seg a) =
+  let l0, l1 = L.splitAt n sg.segment in
+  let sg1 = {segment = l1; exit = sg.exit} in
+  {segment = l0; exit = entry sg1}, sg1
+
+unfold let splitAt_seg_bd (#a:Type) (n:nat) (sg:list_seg a)
+  : Pure (list_seg a & list_seg a)
+         (requires n <= sg_length sg)
+         (ensures fun (sg0,sg1) -> sg_length sg0 = n /\ sg_length sg1 = sg_length sg - n)
+  = L.splitAt_length n sg.segment;
+    splitAt_seg n sg
+
+let splitAt_append_seg (#a:Type) (n:nat) (sg:list_seg a)
+  : Lemma (let sg0,sg1 = splitAt_seg n sg in append_seg sg0 sg1 == sg)
+  = Ll.lemma_splitAt_append n sg.segment
+
+let splitAt_seg_wf (#a : Type) (n:nat) (sg : list_seg a)
+  : Lemma (let sg0,sg1 = splitAt_seg n sg in
+          (wf_seg sg <==> wf_seg sg0 /\ wf_seg sg1 /\ M.loc_disjoint (loc_seg sg0) (loc_seg sg1)))
+  = splitAt_append_seg n sg
+
+let splitAt_seg_live (#a:Type) (n:nat) (h : HS.mem) (sg:list_seg a)
+  : Lemma (let sg0,sg1 = splitAt_seg n sg in
+          (live_seg h sg <==> live_seg h sg0 /\ live_seg h sg1))
+  = splitAt_append_seg n sg
+
+let splitAt_seg_entry (#a:Type) (n:nat) (sg:list_seg a)
+  : Lemma (entry (splitAt_seg n sg)._1 == entry sg)
+  = ()
+
+let rec splitAt_next (#a : Type) (i : nat) (sg : list_seg a)
+  : Lemma (requires i < sg_length sg)
+          (ensures  (splitAt_seg_bd (i + 1) sg)._2 == tail_seg (splitAt_seg_bd i sg)._2)
+          (decreases i)
+  = if i = 0 then () else splitAt_next (i - 1) (tail_seg sg)
+
+let rec splitAt_next_live (#a : Type) (i : nat) (sg : list_seg a) (h : HS.mem)
+  : Lemma (requires live_seg h sg /\ i < sg_length sg)
+          (ensures (let sg1 = (splitAt_seg_bd i sg)._2 in
+                    let ptr = entry sg1 in
+                    Cons? sg1.segment /\
+                    (splitAt_seg_bd (i+1) sg)._2 == tail_seg sg1 /\
+                    ~(B.g_is_null ptr) /\ B.live h ptr /\
+                    (B.deref h ptr).next == entry (tail_seg sg1)))
+          (decreases i)
+  = splitAt_seg_live i h sg;
+    if i = 0 then ()
+    else splitAt_next_live (i-1) (tail_seg sg) h
+
+(* [set_seg] *)
+
+let set_seg (#a : Type) (i : nat) (x : a) (sg : list_seg a)
+  : Pure (list_seg a) (requires i < sg_length sg) (ensures fun sg' -> sg_length sg' = sg_length sg)
+  = { sg with segment = Ll.map_index i (fun (c, _) -> (c, x)) sg.segment }
+
+let rec set_seg_splitAt (#a : Type) (i j : nat) (x : a) (sg : list_seg a)
+  : Lemma (requires i + j < sg_length sg)
+          (ensures  set_seg (i + j) x sg
+                    == (let sg0,sg1 = splitAt_seg_bd i sg in
+                        append_seg sg0 (set_seg j x sg1)))
+          (decreases i)
+  = if i = 0 then ()
+    else (set_seg_splitAt (i-1) j x (tail_seg sg);
+          L.splitAt_length i sg.segment)
+
+(* [reverse_seg] *)
+
+let reverse_seg (#a : Type) (sg : list_seg a) =
+  { segment = L.rev sg.segment; exit = B.null }
+
+let reverse_seg_loc (#a : Type) (sg : list_seg a)
+  : Lemma (ensures loc_seg (reverse_seg sg) == loc_seg sg)
+    [SMTPat (loc_seg (reverse_seg sg))]
+  =
+    loc_seg_fold (reverse_seg sg);
+    loc_seg_fold sg;
+    loc_seg_fold_f_comm a;
+    Ll.fold_right_gtot_comm_permutation_t _ _ (loc_seg_fold_f #a)
+                 M.loc_none (Ll.permutation_t_rev' sg.segment);
+    L.rev_rev' sg.segment
+
+
+(** Manipulation des segments *)
+
+noextract let empty_list (a : Type0) : list_nil a = { segment = []; exit = B.null }
+let empty_live (a : Type0) (h : HS.mem) : Lemma (live_seg h (empty_list a)) = ()
+
+let list_nil_entry_live (#a : Type0) (h : HS.mem) (sg : list_nil a)
+  : Lemma (requires live_seg h sg)
+          (ensures  B.live h (entry sg))
+  = ()
+
+let list_seg_Cons_entry_live (#a : Type0) (h : HS.mem) (sg : list_seg a)
+  : Lemma (requires live_seg h sg /\ Cons? sg.segment)
+          (ensures  B.live h (entry sg))
+  = ()
+
+let entry_null_is_empty (#a : Type0) (h : HS.mem) (sg : list_seg a)
+  : Lemma (requires live_seg h sg /\ entry sg == B.null)
+          (ensures  sg == empty_list a)
+          [SMTPat (live_seg h sg); SMTPat (entry sg == B.null)]
+  = ()
+
+let list_nil_entry_nnull (#a : Type0) (h : HS.mem) (sg : list_nil a)
+  : Lemma (requires live_seg h sg /\ entry sg =!= B.null)
+          (ensures  Cons? sg.segment)
+          [SMTPat (live_seg h sg); SMTPat (Cons? sg.segment)]
+  = ()
+
+
+inline_for_extraction
+let sgn_entry (#a : Type) (p : t a) (sg : G.erased (list_nil a))
+  : Stack (t a) (requires fun h0       -> live_seg h0 sg /\ p == entry sg)
+                (ensures  fun h0 p' h1 -> h0 == h1 /\ B.live h1 p /\ p' == p)
+  = p
+
+inline_for_extraction
+let sg_next (#a : Type) (p : t a) (sg : G.erased (list_seg a))
+  : Stack (t a) (requires fun h0       -> live_seg h0 sg /\ p == entry sg /\ Cons? sg.segment)
+                (ensures  fun h0 p' h1 -> h0 == h1 /\
+                                       live_seg h1 (tail_seg sg) /\ p' == entry (tail_seg sg))
+  = (p.(0ul)).next
